WellScoped.subcapt green again

Capless/CaptureSet.lean
@@ -15,7 +15,6 @@ This file contains the definition of capture sets.
 inductive Singleton : Nat -> Nat -> Type where
 | var : Fin n -> Singleton n k
 | cvar : Fin k -> Singleton n k
-| proj : Singleton n k -> Kind -> Singleton n k
 
 /-- Capture sets in System Capless.
 
@@ -35,21 +34,25 @@ Since the capture sets are indexed with the number of available binders, and eac
 inductive CaptureSet : Nat -> Nat -> Type where
 | empty : CaptureSet n k
 | union : CaptureSet n k -> CaptureSet n k -> CaptureSet n k
-| singleton : Singleton n k -> CaptureSet n k
+| singleton : Singleton n k -> Kind -> CaptureSet n k
 
 @[simp]
 def CaptureSet.proj (c : CaptureSet n k) (K : Kind) :=
   match c with
   | empty => empty
   | union c1 c2 => union (c1.proj K) (c2.proj K)
-  | singleton s => singleton $ s.proj K
+  | singleton s p => singleton s (p.intersect K)
+
+theorem CaptureSet.proj_top {C : CaptureSet n k} : C.proj .top = C := by
+  induction C <;> try aesop
+  apply Kind.Intersect.top_r
 
 @[simp]
 instance : EmptyCollection (CaptureSet n k) where
   emptyCollection := CaptureSet.empty
 
-notation:max "{x=" x "}" => CaptureSet.singleton (Singleton.var x)
-notation:max "{c=" c "}" => CaptureSet.singleton (Singleton.cvar c)
+notation:max "{x=" x " | " K "}" => CaptureSet.singleton (Singleton.var x) K
+notation:max "{c=" c " | " K "}" => CaptureSet.singleton (Singleton.cvar c) K
 
 @[simp]
 instance : Union (CaptureSet n k) where
@@ -120,14 +123,12 @@ def Singleton.rename (s : Singleton n k) (f : FinFun n n') : Singleton n' k :=
   match s with
   | var n => var $ f n
   | cvar k => cvar k
-  | proj s K => (s.rename f).proj K
 
 @[simp]
 def Singleton.crename (s : Singleton n k) (f : FinFun k k') : Singleton n k' :=
   match s with
   | var n => var n
   | cvar k => cvar $ f k
-  | proj s K => (s.crename f).proj K
 
 @[simp]
 theorem Singleton.rename_id {s : Singleton n k} :
@@ -159,14 +160,14 @@ def CaptureSet.rename (C : CaptureSet n k) (f : FinFun n n') : CaptureSet n' k :
   match C with
   | empty => empty
   | union C1 C2 => (C1.rename f) ∪ (C2.rename f)
-  | singleton s => singleton $ s.rename f
+  | singleton s p => singleton (s.rename f) p
 
 @[simp]
 def CaptureSet.crename (C : CaptureSet n k) (f : FinFun k k') : CaptureSet n k' :=
   match C with
   | empty => empty
   | union C1 C2 => (C1.crename f) ∪ (C2.crename f)
-  | singleton s => singleton $ s.crename f
+  | singleton s p => singleton (s.crename f) p
 
 def CaptureSet.weaken (C : CaptureSet n k) : CaptureSet (n+1) k :=
   C.rename FinFun.weaken
@@ -201,20 +202,20 @@ theorem CaptureSet.cweaken_union {C1 C2 : CaptureSet n k} :
   simp [CaptureSet.cweaken, CaptureSet.crename_union]
 
 theorem CaptureSet.rename_singleton {x : Fin n} {f : FinFun n n'} :
-  ({x=x} : CaptureSet n k).rename f = {x=f x} := by simp
+  ({x=x | K} : CaptureSet n k).rename f = {x=f x | K} := by simp
 
 theorem CaptureSet.ext_rename_singleton_zero {f : FinFun n n'} :
-  ({x=0} : CaptureSet (n+1) k).rename f.ext = {x=0} := by
+  ({x=0 | K} : CaptureSet (n+1) k).rename f.ext = {x=0 | K} := by
   simp [FinFun.ext]
 
 theorem CaptureSet.rename_csingleton {x : Fin k} {f : FinFun n n'} :
-  {c=x}.rename f = {c=x} := by simp
+  {c=x | K}.rename f = {c=x | K} := by simp
 
 theorem CaptureSet.crename_singleton {x : Fin n} {f : FinFun k k'} :
-  {x=x}.crename f = {x=x} := by simp
+  {x=x | K}.crename f = {x=x | K} := by simp
 
 theorem CaptureSet.crename_csingleton {x : Fin k} {f : FinFun k k'} :
-  ({c=x} : CaptureSet n k).crename f = {c=f x} := by simp
+  ({c=x | K} : CaptureSet n k).crename f = {c=f x | K} := by simp
 
 theorem CaptureSet.rename_empty :
   ({} : CaptureSet n k).rename f = {} := by simp
@@ -260,11 +261,11 @@ theorem CaptureSet.cweaken_crename {C : CaptureSet n k} :
   simp [cweaken, crename_crename, FinFun.comp_weaken]
 
 theorem CaptureSet.cweaken_csingleton {c : Fin k} :
-  ({c=c} : CaptureSet n k).cweaken = {c=c.succ} := by
+  ({c=c | K} : CaptureSet n k).cweaken = {c=c.succ | K} := by
   simp [singleton, cweaken, crename, FinFun.weaken]
 
 theorem CaptureSet.weaken_csingleton :
-  ({c=c} : CaptureSet n k).weaken = {c=c} := by
+  ({c=c | K} : CaptureSet n k).weaken = {c=c | K} := by
   simp [singleton, weaken]
 
 theorem CaptureSet.rename_id {C : CaptureSet n k} :
@@ -309,79 +310,6 @@ theorem CaptureSet.cweaken_def {C : CaptureSet n k} :
 -- ## Projections
 -- -/
 
--- `n` with projections widen `C'` to given `C`
-inductive WidenVar : Fin n -> Singleton n k -> CaptureSet n k -> CaptureSet n k -> Prop where
-  | var : WidenVar x (.var x) C C
-  | proj : WidenVar n s C' C -> WidenVar n (s.proj K) C' (C.proj K)
-
--- `n` with projections widen to given `C`, including a projection to `K`
-inductive WidenVarWith : Fin n -> Singleton n k -> CaptureSet n k -> CaptureSet n k -> Kind -> Prop where
-  | here : WidenVar n s C' C -> WidenVarWith n (s.proj K) C' (C.proj K) K
-  | there : WidenVarWith n s C' C K -> WidenVarWith n (s.proj K') C' (C.proj K') K
-
--- `k` with projections widen `C'` to given `C`
-inductive WidenCVar : Fin k -> Singleton n k -> CaptureSet n k -> CaptureSet n k -> Prop where
-  | var : WidenCVar c (.cvar c) C C
-  | proj : WidenCVar c s C' C -> WidenCVar c (s.proj K) C' (C.proj K)
-
--- `k` with projections widen to given `C`, including a projection to `K`
-inductive WidenCVarWith : Fin k -> Singleton n k -> CaptureSet n k -> CaptureSet n k -> Kind -> Prop where
-  | here : WidenCVar c s C' C -> WidenCVarWith c (s.proj K) C' (C.proj K) K
-  | there : WidenCVarWith c s C' C K -> WidenCVarWith c (s.proj K') C' (C.proj K') K
-
-inductive Singleton.IsVar : Singleton n k -> Fin n -> Prop where
-  | var : IsVar (.var x) x
-  | proj : IsVar s x -> IsVar (s.proj K) x
-
-theorem Singleton.IsVar.proj_inv (hv : IsVar (s.proj K) n) : IsVar s n := by cases hv; assumption
-
-theorem WidenVar.is_var (hw : WidenVar n s C' C) : s.IsVar n := by
-  induction hw
-  case var => constructor
-  case proj ih => apply ih.proj
-
-inductive Singleton.IsVarWith : Singleton n k -> Fin n -> Kind -> Prop where
-  | here : IsVar s n -> IsVarWith (s.proj K) n K
-  | there : IsVarWith s n K -> IsVarWith (s.proj K') n K
-
-theorem WidenVarWith.is_var_with (hw : WidenVarWith k s C' C K) : s.IsVarWith k K := by
-  induction hw
-  case here hw => apply Singleton.IsVarWith.here hw.is_var
-  case there ih => apply ih.there
-
-inductive Singleton.IsAbsurdVar : Singleton n k -> Fin n -> Prop where
-  | here : K1.Disjoint K2 -> s.IsVarWith x K1 -> IsAbsurdVar (.proj s K2) x
-  | there : IsAbsurdVar s x -> IsAbsurdVar (s.proj K) x
-
-inductive Singleton.IsCVar : Singleton n k -> Fin k -> Prop where
-  | var : IsCVar (.cvar n) n
-  | proj : IsCVar s n -> IsCVar (s.proj K) n
-
-theorem Singleton.IsCVar.proj_inv (hv : IsCVar (s.proj K) n) : IsCVar s n := by cases hv; assumption
-
-theorem WidenCVar.is_cvar (hw : WidenCVar n s C' C) : s.IsCVar n := by
-  induction hw
-  case var => constructor
-  case proj ih => apply ih.proj
-
-theorem CaptureSet.proj_singleton : (singleton s).proj K = (singleton $ s.proj K) := by simp
-
-theorem CaptureSet.proj_inj {C D : CaptureSet n k} (heq : C.proj K = D.proj K) : C = D := by
-  induction C generalizing D
-  case empty =>
-    simp at heq
-    unfold proj at heq; split at heq <;> simp at heq
-    rfl
-  case union ha hb =>
-    simp at heq
-    cases D <;> simp at heq
-    have ⟨_, _⟩ := heq
-    rw [ha _, hb _]
-    repeat assumption
-  case singleton =>
-    cases D <;> simp at heq
-    aesop
-
 theorem CaptureSet.Subset.proj (hsub : Subset C D) : Subset (C.proj K) (D.proj K) := by
   induction hsub <;> try simp
   case empty => apply empty
@@ -389,220 +317,3 @@ theorem CaptureSet.Subset.proj (hsub : Subset C D) : Subset (C.proj K) (D.proj K
   case union_l ha hb => apply! union_l
   case union_rl ha => apply! union_rl
   case union_rr hb => apply! union_rr
-
--- inductive HasSingleton : Singleton n k -> Singleton n k -> Prop where
---   | var : HasSingleton (.var n) (.var n)
---   | cvar : HasSingleton (.cvar k) (.cvar k)
---   | proj : HasSingleton s s' -> HasSingleton (.proj s K) s'
-
--- inductive HasSingletonProj : Singleton n k -> Singleton n k -> Kind -> Prop where
---   | here : HasSingleton s s' -> HasSingletonProj (.proj s K) s' K
---   | there : HasSingletonProj s s' K -> HasSingletonProj (.proj s K') s' K
-
--- theorem HasSingleton.is_not_proj (hh : HasSingleton s (.proj s' K)) : False := by
---   cases hh
---   case proj hh => apply hh.is_not_proj
-
--- theorem HasSingleton.is_target (hs1 : HasSingleton s t) (hs2 : HasSingleton t u) : t = u := by
---   induction hs1
---   case var => cases hs2; rfl
---   case cvar => cases hs2; rfl
---   case proj ih => apply! ih
-
--- theorem HasSingletonProj.erase (hs : HasSingletonProj s s' K) : HasSingleton s s' := by
---   induction hs
---   case here => apply! HasSingleton.proj
---   case there ih => apply! HasSingleton.proj
-
--- inductive ProjectedSingleton: CaptureSet n k -> (CaptureSet n k) -> Prop where
---   | var : ProjectedSingleton {x=x} {x=x}
---   | cvar : ProjectedSingleton {c=c} {c=c}
---   | proj : ProjectedSingleton s C -> ProjectedSingleton s (.proj C K)
-
--- inductive ProjectedSingletonWith : (CaptureSet n k) -> (K : Kind) -> (CaptureSet n k) -> Prop where
---   | here : ProjectedSingleton s C -> ProjectedSingletonWith s K (.proj C K)
---   | there : ProjectedSingletonWith s K C -> ProjectedSingletonWith s K (.proj C K')
-
--- def ProjectedSingletonWith.erase (hp : ProjectedSingletonWith s K C) : ProjectedSingleton s C := by
---   induction hp <;> apply! ProjectedSingleton.proj
-
--- /-- A capture set that only has projections on top of singletons. -/
--- inductive ProjectedSingletonsOnly: CaptureSet n k -> Prop where
---   | empty : ProjectedSingletonsOnly .empty
---   | singleton : ProjectedSingleton s C -> ProjectedSingletonsOnly C
---   | union : ProjectedSingletonsOnly C1 -> ProjectedSingletonsOnly C2 -> ProjectedSingletonsOnly (.union C1 C2)
-
--- @[simp]
--- def CaptureSet.push_proj (C: CaptureSet n k) (K: Kind) : CaptureSet n k :=
---   match C with
---   | .empty => .empty
---   | .singleton c => proj (.singleton c) K
---   | .csingleton c => proj (.csingleton c) K
---   | .proj C1 K1 => proj (.proj C1 K1) K
---   | .union C1 C2 => .union (C1.push_proj K) (C2.push_proj K)
-
--- @[simp]
--- def CaptureSet.canonicalize (C : CaptureSet n k) : CaptureSet n k :=
---   match C with
---   | .empty => .empty
---   | .singleton c => .singleton c
---   | .csingleton c => .csingleton c
---   | .union C1 C2 => .union (C1.canonicalize) (C2.canonicalize)
---   | .proj C1 K => C1.canonicalize.push_proj K
-
--- theorem CaptureSet.push_proj_is_superset (C : CaptureSet n k) : (C.proj K) ⊆ C.push_proj K := by
---   induction C <;> simp only [push_proj]
---   case empty => exists 0; apply Subset.proj_empty
---   case union C1 C2 ih1 ih2 =>
---     apply IsTrans.trans (r := HasSubset.Subset)
---     exists 0; apply Subset.proj_union_r
---     apply! Subset.union_monotone
---   case singleton => exists 0; apply Subset.rfl
---   case csingleton => exists 0; apply Subset.rfl
---   case proj => apply Subset.proj' Subset.rfl'
-
--- theorem CaptureSet.canonicalize_is_superset {C : CaptureSet n k} : C ⊆ C.canonicalize := by
---   induction C <;> (simp; try apply Subset.rfl')
---   case union ih1 ih2 => apply Subset.union_monotone ih1 ih2
---   case proj C1 K ih =>
---     apply Subset.trans'
---     apply Subset.proj' ih
---     apply push_proj_is_superset
-
--- theorem CaptureSet.push_proj_is_subset {C : CaptureSet n k} : C.push_proj K ⊆ C.proj K := by
---   induction C <;> (simp; try apply Subset.rfl')
---   case empty => apply Subset.empty'
---   case union C1 C2 ih1 ih2 =>
---     apply Subset.trans' _ Subset.proj_union_l'
---     apply! Subset.union_monotone
-
--- theorem CaptureSet.canonicalize_is_subset {C : CaptureSet n k} : C.canonicalize ⊆ C := by
---   induction C <;> (simp; try apply Subset.rfl')
---   case union ih1 ih2 => apply Subset.union_monotone ih1 ih2
---   case proj C1 K ih =>
---     apply Subset.trans' C1.canonicalize.push_proj_is_subset
---     apply Subset.proj' ih
-
--- theorem CaptureSet.push_proj_singleton {C : CaptureSet n k} (hp: ProjectedSingletonsOnly C) : ProjectedSingletonsOnly (C.push_proj K) := by
---   induction hp <;> try simp_all
---   case empty => constructor
---   case singleton hp =>
---     induction hp
---     case var => apply ProjectedSingletonsOnly.singleton (.proj .var)
---     case cvar => apply ProjectedSingletonsOnly.singleton (.proj .cvar)
---     case proj =>
---       apply ProjectedSingletonsOnly.singleton
---       apply ProjectedSingleton.proj
---       apply! ProjectedSingleton.proj
---   case union C1 C2 ih1 ih2 =>
---     apply! ProjectedSingletonsOnly.union
-
--- theorem CaptureSet.canonicalize_is_projected_singletons_only {C : CaptureSet n k} : ProjectedSingletonsOnly C.canonicalize := by
---   induction C <;> try simp
---   case empty => apply ProjectedSingletonsOnly.empty
---   case singleton => apply ProjectedSingletonsOnly.singleton .var
---   case csingleton => apply ProjectedSingletonsOnly.singleton .cvar
---   case union C1 C2 ih1 ih2 => apply ProjectedSingletonsOnly.union ih1 ih2
---   case proj C K ih =>
---     apply push_proj_singleton
---     assumption
-
--- lemma CaptureSet.push_proj_depth {C : CaptureSet n k} : (C.push_proj K).depth ≤ 1 + C.depth := by
---   induction C <;> simp; omega
-
--- theorem CaptureSet.canonicalize_depth {C : CaptureSet n k} : C.canonicalize.depth ≤ C.depth := by
---   induction C <;> simp
---   case union ih1 ih2 => omega
---   case proj C K ih =>
---     apply IsTrans.trans
---     apply C.canonicalize.push_proj_depth
---     simp; exact ih
-
--- lemma CaptureSet.push_proj_singleton_eq {C : CaptureSet n k} (hp : ProjectedSingleton s C) : (C.push_proj K) = (C.proj K) := by
---   induction hp <;> simp
-
--- theorem CaptureSet.canonicalize_projected_singletons {C : CaptureSet n k} (hp : ProjectedSingletonsOnly C) : C.canonicalize = C := by
---   induction hp
---   case singleton s C hs =>
---     induction hs <;> simp
---     case proj ha ih =>
---       rw [ih]
---       apply! push_proj_singleton_eq
---   case empty => simp
---   case union ha hb iha ihb =>
---     simp; aesop
-
--- theorem CaptureSet.canonicalize_idempt {C : CaptureSet n k} : C.canonicalize.canonicalize = C.canonicalize := by
---   have h := C.canonicalize_is_projected_singletons_only
---   rw [C.canonicalize.canonicalize_projected_singletons h]
-
--- theorem CaptureSet.Subset.canonicalize {A B : CaptureSet n k} (hs : A ⊆ B) : A.canonicalize ⊆ B.canonicalize := by
---   apply trans'
---   apply A.canonicalize_is_subset
---   apply trans' hs
---   apply B.canonicalize_is_superset
-
-
--- inductive HasSingleton : CaptureSet n k -> CaptureSet n k -> Prop where
---   | var : HasSingleton {x=x} {x=x}
---   | cvar : HasSingleton {c=c} {c=c}
---   | union_l : HasSingleton s C1 -> HasSingleton s (.union C1 C2)
---   | union_r : HasSingleton s C2 -> HasSingleton s (.union C1 C2)
---   | proj : HasSingleton s C -> HasSingleton (s.proj K) (C.proj K)
-
--- theorem CaptureSet.Subset.subset_has_singleton' {C1 C2 : CaptureSet n k} (hh1 : HasSingleton s C1) (hs : Subset t C1 C2) : HasSingleton s C2 := by
---   induction hs generalizing s
---   case empty => cases hh1
---   case rfl => assumption
---   case union_l ih1 ih2 =>
---     cases hh1
---     apply! ih1
---     apply! ih2
---   case union_rl ih => apply HasSingleton.union_l; apply ih hh1
---   case union_rr ih => apply HasSingleton.union_r; apply ih hh1
---   case trans ha hb iha ihb =>
---     apply ihb $ iha hh1
---   case proj_empty => cases hh1; rename_i hh1; cases hh1
---   case proj_union_l =>
---     cases hh1
---     { rename_i hh1; cases hh1; constructor; apply! HasSingleton.union_l }
---     { rename_i hh1; cases hh1; constructor; apply! HasSingleton.union_r }
---   case proj_union_r =>
---     cases hh1
---     rename_i hh1
---     cases hh1
---     { apply HasSingleton.union_l; constructor; assumption }
---     { apply HasSingleton.union_r; constructor; assumption }
---   case proj ih =>
---     cases hh1
---     constructor
---     apply! ih
-
--- theorem CaptureSet.subset_has_singleton {C1 C2 : CaptureSet n k} (hs : C1 ⊆ C2) (hh : HasSingleton C C1) : HasSingleton C C2 := by
---   have ⟨_, h⟩ := hs
---   apply Subset.subset_has_singleton' hh h
-
--- theorem CaptureSet.projected_singleton_has_singleton (hp : ProjectedSingleton s C) : HasSingleton C C := by
---   induction hp
---   case var => constructor
---   case cvar => constructor
---   case proj hp => constructor; assumption
-
--- theorem CaptureSet.projected_singleton_unique_singleton (hp : ProjectedSingleton s C) (hh : HasSingleton C' C) : C' = C := by
---   induction hp generalizing C'
---   case var => cases hh; rfl
---   case cvar => cases hh; rfl
---   case proj hp ih =>
---     cases hh
---     rename_i hh
---     have ih1 := ih hh
---     subst_vars
---     simp
-
-
--- theorem CaptureSet.Subset.empty_projected_singleton {C : CaptureSet n k} (hs : C ⊆ .empty) (hp : ProjectedSingleton s C) : False := by
---   have ⟨n, h⟩ := hs
---   have h2 := CaptureSet.Subset.subset_has_singleton' (projected_singleton_has_singleton hp) h
---   cases h2
-
--- end Capless
