Capless/WellScoped/Basic.lean
@@ -11,17 +11,94 @@ This file contains basic properties of the well-scopedness relation.
 
 namespace Capless
 
-theorem WellScoped.proj (hsc : WellScoped Γ cont C) : WellScoped Γ cont (C.proj K) := by
-  induction hsc generalizing K <;> simp
-  case empty => apply empty
-  case union iha ihb => apply union iha ihb
-  case singleton hb hw hsc ih => apply singleton hb hw.proj ih
-  case csingleton hb hw hsc ih => apply csingleton hb hw.proj ih
-  case cbound hb hw hsc ih => apply cbound hb hw.proj ih
-  case ckind hb hw => apply ckind hb hw.proj
-  case label hb hl hw => apply label hb hl hw.proj
-  case label_disj hb hd hw => apply label_disj hb hd hw.there
-  case label_absurd hb ha => apply label_absurd hb ha.there
+theorem WellScoped.subkind
+  (hsc : WellScoped Γ cont (.proj C K2))
+  (hs : K1.Subkind K2)
+  : WellScoped Γ cont (.proj C K1) := by
+  generalize h : C.proj K2 = D at hsc
+  induction hsc generalizing C K2 K1
+  case empty =>
+    unfold CaptureSet.proj at h; split at h <;> simp at h
+    simp; constructor
+  case union ha hb =>
+    unfold CaptureSet.proj at h; split at h <;> simp at h
+    have ⟨_, _⟩ := h; subst_vars; simp_all
+    apply! union (ha _ $ .refl _) (hb _ $ .refl _)
+  case singleton hb hsc ih =>
+    unfold CaptureSet.proj at h; split at h <;> simp at h
+    have ⟨_, _⟩ := h; subst_vars; simp_all
+    apply singleton hb
+    apply ih
+    apply Kind.Intersect.with_subkind hs
+    apply! refl
+  case csingleton hb hsc ih =>
+    unfold CaptureSet.proj at h; split at h <;> simp at h
+    have ⟨_, _⟩ := h; subst_vars; simp_all
+    apply csingleton hb
+    apply ih
+    apply Kind.Intersect.with_subkind hs
+    apply! refl
+  case cbound hb hsc ih =>
+    unfold CaptureSet.proj at h; split at h <;> simp at h
+    have ⟨_, _⟩ := h; subst_vars; simp_all
+    apply cbound hb
+    apply ih
+    apply Kind.Intersect.with_subkind hs
+    apply! refl
+  case ckind hb ih =>
+    unfold CaptureSet.proj at h; split at h <;> simp at h
+    have ⟨_, _⟩ := h; subst_vars; simp_all
+    apply! ckind
+  case label hb hl =>
+    unfold CaptureSet.proj at h; split at h <;> simp at h
+    have ⟨_, _⟩ := h; subst_vars; simp_all
+    apply! label
+  case label_disj hb hd =>
+    unfold CaptureSet.proj at h; split at h <;> simp at h
+    have ⟨_, _⟩ := h; subst_vars; simp_all
+    apply label_disj hb
+    apply hd.refine_subkind_l $ Kind.Intersect.with_subkind hs
+  case absurd he =>
+    unfold CaptureSet.proj at h; split at h <;> simp at h
+    have ⟨_, _⟩ := h; subst_vars; simp_all
+    apply absurd
+    apply (Kind.Intersect.with_subkind hs).of_empty he
+
+theorem WellScoped.subkind_singleton
+  (hsc : WellScoped Γ cont (.singleton s L))
+  (hs : Kind.Subkind K L)
+  : WellScoped Γ cont (.singleton s K) := by
+  rw [← Kind.Intersect.top_l (K:=L)] at hsc
+  have h : CaptureSet.proj (.singleton s .top) L = .singleton s (.intersect .top L) := by simp
+  rw [← h] at hsc
+  have h1 := hsc.subkind hs
+  simp only [CaptureSet.proj] at h1
+  rw [Kind.Intersect.top_l] at h1
+  assumption
+
+-- theorem WellScoped.proj (hsc : WellScoped Γ cont C) : WellScoped Γ cont (C.proj K) := by
+--   induction hsc generalizing K
+--   case empty => apply empty
+--   case union ih1 ih2 => apply union ih1 ih2
+--   case singleton hb hsc ih =>
+--     simp only [CaptureSet.proj]
+--     apply singleton hb ih
+--   case csingleton hb hsc ih =>
+--     simp only [CaptureSet.proj]
+--     apply csingleton hb ih
+--   case cbound hb hsc ih =>
+--     simp only [CaptureSet.proj]
+--     apply cbound hb ih
+--   case ckind hb =>
+--     simp only [CaptureSet.proj]
+--     apply ckind hb
+--   case label hb hl =>
+--     simp only [CaptureSet.proj]
+--     apply label hb hl
+--   case label_disj hb hd =>
+--     simp only [CaptureSet.proj]
+--     apply label_disj hb (hd.intersect_disjoint Kind.Intersect.lawful)
+
 
 theorem WellScoped.subset {C1 C2 : CaptureSet n k}
   (hsc : WellScoped Γ cont C2)
@@ -48,13 +125,12 @@ theorem WellScoped.cons
   case csingleton ih => apply csingleton <;> aesop
   case cbound ih => apply cbound <;> aesop
   case ckind ih => apply ckind <;> aesop
-  case label hb hl hw =>
+  case label hb hl =>
     apply label hb
     constructor; assumption
-    apply hw
   case label_disj hb hd =>
     apply! label_disj
-  case label_absurd => apply! label_absurd
+  case absurd => apply! absurd
 
 theorem WellScoped.conse
   (hsc : WellScoped Γ cont C) :
@@ -66,12 +142,11 @@ theorem WellScoped.conse
   case csingleton ih => apply csingleton <;> aesop
   case cbound ih => apply cbound <;> aesop
   case ckind ih => apply ckind <;> aesop
-  case label hb hl hw =>
+  case label hb hl =>
     apply label hb
     constructor; assumption
-    apply hw
   case label_disj => apply! label_disj
-  case label_absurd => apply! label_absurd
+  case absurd => apply! absurd
 
 theorem WellScoped.scope
   (hsc : WellScoped Γ cont C) :
@@ -83,133 +158,133 @@ theorem WellScoped.scope
   case csingleton ih => apply csingleton <;> aesop
   case cbound ih => apply cbound <;> aesop
   case ckind ih => apply ckind <;> aesop
-  case label hb hl hw =>
+  case label hb hl =>
     apply label hb
     constructor; assumption
-    apply hw
   case label_disj => apply! label_disj
-  case label_absurd => apply! label_absurd
+  case absurd => apply! absurd
 
-theorem WellScoped.subkind' {C D : CaptureSet n k}
-  (hsc : WellScoped Γ cont D)
-  (heq : D = C.proj K2)
-  (hs : K1.Subkind K2)
-  : WellScoped Γ cont (C.proj K1) := by
-  induction hsc generalizing C <;> (unfold CaptureSet.proj at heq; split at heq <;> simp at heq; simp)
-  { apply empty }
-  { have ⟨_, _⟩ := heq; subst_vars;
-    rename_i ih1 _ ih2
-    apply union (ih1 _) (ih2 _) <;> rfl }
-  { subst_vars
-    rename_i hw
-    cases hw
-    rename_i hb _ _ _ hw hsc ih
-    apply singleton hb (.proj hw) (ih _)
-    rfl }
-  { subst_vars
-    rename_i hw
-    cases hw
-    rename_i hb _ _ _ hw hsc ih
-    apply csingleton hb (.proj hw) (ih _)
-    rfl }
-  { subst_vars
-    rename_i hw
-    cases hw
-    rename_i hb _ _ _ hw hsc ih
-    apply cbound hb (.proj hw) (ih _)
-    rfl }
-  { subst_vars
-    rename_i hw
-    apply! ckind _ hw.proj_inv.proj }
-  { subst_vars
-    rename_i hw
-    apply! label _ _ hw.proj_inv.proj }
-  { subst_vars
-    rename_i hw
-    cases hw
-    case here hw => apply! label_disj _ (hw.refine_by_subkind _) (.here _)
-    case there hw => apply! label_disj _ _ (.there _) }
-  { subst_vars
-    rename_i hb _ _ hw
-    cases hw
-    case here hd hw =>
-      apply label_absurd hb (.here _ hw)
-      apply! (hd.symm.refine_by_subkind _).symm
-    case there hw => apply! label_absurd hb (.there _) }
+theorem WellScoped.absurd_set
+  (he : Kind.IsEmpty L)
+  : WellScoped Γ cont (.proj C L) := by
+  induction C
+  case empty => simp; constructor
+  case union ha hb => simp; apply! union
+  case singleton =>
+    simp
+    apply absurd
+    apply! Kind.Subkind.of_empty Kind.Intersect.subkind_r
 
-theorem WellScoped.subkind {C: CaptureSet n k} (hsc : WellScoped Γ cont (C.proj K2)) (hs : K1.Subkind K2) : WellScoped Γ cont (C.proj K1) := by
-  apply subkind' hsc _ hs
-  rfl
+theorem WellScoped.proj_merge
+  (hsc1 : WellScoped Γ cont (.proj C K1))
+  (hsc2 : WellScoped Γ cont (.proj C K2))
+  : WellScoped Γ cont (.proj C (K1.union K2)) := by
+  generalize h : C.proj K1 = D at hsc1
+  induction hsc1 generalizing C K1 K2
+  case empty =>
+    unfold CaptureSet.proj at h; split at h <;> simp at h
+    simp; constructor
+  case union ha hb =>
+    unfold CaptureSet.proj at h; split at h <;> simp at h
+    have ⟨_, _⟩ := h; subst_vars; simp_all
+    cases hsc2
+    apply! union (ha _ $ .refl _) (hb _ $ .refl _)
+  case singleton hb hsc ih =>
+    unfold CaptureSet.proj at h; split at h <;> simp at h
+    have ⟨_, _⟩ := h; subst_vars; simp_all
+    cases hsc2
+    case singleton hb2 hsc2 =>
+      cases Context.bound_injective hb hb2
+      apply singleton hb
+      apply subkind _ Kind.Intersect.union_r_subkind
+      apply! ih _ (.refl _)
+    case label hb2 _ => cases Context.bound_lbound_absurd hb hb2
+    case label_disj hb2 _ => cases Context.bound_lbound_absurd hb hb2
+    case absurd p he =>
+      have h : (p.intersect (K1.union K2)).Subkind (p.intersect K1) := by
+        apply Kind.Subkind.trans Kind.Intersect.union_r_subkind
+        apply Kind.Subkind.union_l .rfl
+        apply! Kind.Subkind.is_empty_l
+      apply subkind_singleton _ h
+      apply! singleton
+  case csingleton hb hsc ih =>
+    unfold CaptureSet.proj at h; split at h <;> simp at h
+    have ⟨_, _⟩ := h; subst_vars; simp_all
+    cases hsc2
+    case csingleton hb2 hsc2 =>
+      cases Context.cbound_injective hb hb2
+      apply csingleton hb
+      apply subkind _ Kind.Intersect.union_r_subkind
+      apply! ih _ (.refl _)
+    case cbound hb2 _ => cases Context.cbound_injective hb hb2
+    case ckind hb2 => cases Context.cbound_injective hb hb2
+    case absurd p he =>
+      have h : (p.intersect (K1.union K2)).Subkind (p.intersect K1) := by
+        apply Kind.Subkind.trans Kind.Intersect.union_r_subkind
+        apply Kind.Subkind.union_l .rfl
+        apply! Kind.Subkind.is_empty_l
+      apply subkind_singleton _ h
+      apply! csingleton
+  case cbound hb hsc ih =>
+    unfold CaptureSet.proj at h; split at h <;> simp at h
+    have ⟨_, _⟩ := h; subst_vars; simp_all
+    cases hsc2
+    case csingleton hb2 _ => cases Context.cbound_injective hb hb2
+    case cbound hb2 hsc2 =>
+      cases Context.cbound_injective hb hb2
+      apply cbound hb
+      apply subkind _ Kind.Intersect.union_r_subkind
+      apply! ih _ (.refl _)
+    case ckind hb2 => cases Context.cbound_injective hb hb2
+    case absurd p he =>
+      have h : (p.intersect (K1.union K2)).Subkind (p.intersect K1) := by
+        apply Kind.Subkind.trans Kind.Intersect.union_r_subkind
+        apply Kind.Subkind.union_l .rfl
+        apply! Kind.Subkind.is_empty_l
+      apply subkind_singleton _ h
+      apply! cbound
+  case ckind hb =>
+    unfold CaptureSet.proj at h; split at h <;> simp at h
+    have ⟨_, _⟩ := h; subst_vars; simp_all
+    apply! ckind
+  case label hb hl =>
+    unfold CaptureSet.proj at h; split at h <;> simp at h
+    have ⟨_, _⟩ := h; subst_vars; simp_all
+    apply! label
+  case label_disj hb hd =>
+    unfold CaptureSet.proj at h; split at h <;> simp at h
+    have ⟨_, _⟩ := h; subst_vars; simp_all
+    cases hsc2
+    case singleton hb2 _ => cases Context.bound_lbound_absurd hb2 hb
+    case label hb hl => apply! label
+    case label_disj hb2 hd2 =>
+      cases Context.lbound_inj hb hb2
+      subst_vars
+      have h := Kind.Disjoint.union_l hd hd2
+      apply subkind_singleton (label_disj hb h) Kind.Intersect.union_r_subkind
+    case absurd he =>
+      have h := Kind.Disjoint.union_l hd (.is_empty_l he)
+      apply subkind_singleton (label_disj hb h) Kind.Intersect.union_r_subkind
+  case absurd he =>
+    unfold CaptureSet.proj at h; split at h <;> simp at h
+    have ⟨_, _⟩ := h; subst_vars; simp_all
+    rename_i p
+    have h : (p.intersect (K1.union K2)).Subkind (p.intersect K2) := by
+      apply Kind.Subkind.trans Kind.Intersect.union_r_subkind
+      apply Kind.Subkind.union_l _ .rfl
+      apply Kind.Subkind.is_empty_l he
+    apply! subkind_singleton _ h
 
--- theorem WellScoped.capture_kind'
---   (hsc : WellScoped Γ cont D)
---   (heq : D = C.proj K)
---   (hk : CaptureKind Γ C K)
---   : WellScoped Γ cont C := by
---   induction hsc generalizing C <;> (unfold CaptureSet.proj at heq; split at heq <;> simp at heq)
---   { apply empty }
---   { have ⟨_, _⟩ := heq; subst_vars
---     rename_i h1 ih1 h2 ih2
---     have ⟨_, _⟩ := hk.union_l_inv
---     -- apply union (ih1 _ hk) (ih2 _ hk)
---     apply! union (ih1 (.refl _) _) (ih2 (.refl _) _) }
---   { rename_i hb hw hsc ih _ _;
---     subst_vars;
---     cases hw;
---     apply singleton hb
---     assumption
---     apply ih (.refl _)
---     apply hk.widen_var hb
---     assumption }
---   { rename_i hb hw hsc ih _ _;
---     subst_vars;
---     cases hw;
---     apply csingleton hb
---     assumption
---     apply ih (.refl _)
---     apply hk.widen_cinstr hb
---     assumption }
---   { rename_i hb hw hsc ih _ _;
---     subst_vars;
---     cases hw;
---     apply cbound hb
---     assumption
---     apply ih (.refl _)
---     apply hk.widen_cbound hb
---     assumption }
---   { rename_i hb hi _ _
---     cases hi <;> cases heq
---     apply! ckind
---   }
---   { rename_i hb hl hi _ _
---     cases hi <;> cases heq
---     apply! label }
---   { rename_i hb hd hi _ _
---     cases hi <;> cases heq
---     case here.refl hi =>
---       cases hk.widen_lbound hb hi
---       case inl hsub => cases Kind.subkind_disjoint_absurd hsub hd.symm
---       case inr hi =>
---         have ⟨K1, _, hi⟩ := hi
---         apply label_disj hb _ hi
---         apply! hd.refine_by_subkind
---     case there.refl hi => apply! label_disj
---   }
+theorem WellScoped.proj_merge_singleton
+  (hs1 : WellScoped Γ cont (.singleton s K1))
+  (hs2 : WellScoped Γ cont (.singleton s K2))
+  : WellScoped Γ cont (.singleton s (K1.union K2)) := by
+  rw [← Kind.Intersect.top_l (K:=K1)] at hs1
+  rw [← Kind.Intersect.top_l (K:=K2)] at hs2
+  rw [← CaptureSet.proj] at hs1 hs2
+  rw [← Kind.Intersect.top_l (K:=K1.union K2), ← CaptureSet.proj]
+  apply! proj_merge
 
--- theorem WellScoped.capture_kind (hsc : WellScoped Γ cont (C.proj K)) (hk : CaptureKind Γ C K) : WellScoped Γ cont C := by apply! hsc.capture_kind' $ .refl _
-
-theorem WellScoped.union_inv (hsc : WellScoped Γ cont (C1 ∪ C2)) : WellScoped Γ cont C1 ∧ WellScoped Γ cont C2 := by
-  cases hsc; aesop
-
-theorem WellScoped.singleton_inv (hsc : WellScoped Γ cont {x=x}) (hb : Γ.Bound x S^C) : WellScoped Γ cont C := by
-  cases hsc
-  case singleton hb1 hs hw => cases hw; cases Context.bound_injective hb hb1; assumption
-  case csingleton hw => cases hw
-  case cbound hw => cases hw
-  case ckind hw => cases hw
-  case label hb1 _ hw => cases hw; cases Context.bound_lbound_absurd hb hb1
-  case label_disj hb1 _ hw => cases hw
-  case label_absurd hb1 _ hw => cases hw
 
 theorem WellScoped.subcapt (hsc : WellScoped Γ cont C2) (hsub : Subcapt Γ C1 C2) : WellScoped Γ cont C1 := by
   induction hsub
@@ -217,205 +292,27 @@ theorem WellScoped.subcapt (hsc : WellScoped Γ cont C2) (hsub : Subcapt Γ C1 C
   case subset hsub => apply! hsc.subset
   case union ha hb iha ihb =>
     apply! union (iha _) (ihb _)
-  case var hb => apply! singleton _ .var
+  case var hb => apply! singleton
   case cinstl hb =>
     cases hsc
-    case singleton hv => cases hv
-    case csingleton hb1 _ hv =>
-      cases hv
+    case csingleton hb1 _ =>
       cases Context.cbound_injective hb1 hb
       assumption
-    case cbound hb1 _ hv =>
-      cases hv
+    case cbound hb1 _ =>
       cases Context.cbound_injective hb1 hb
-    case ckind hb1 hv =>
-      cases hv
+    case ckind hb1 =>
       cases Context.cbound_injective hb1 hb
-    case label hv => cases hv
-    case label_disj hv => cases hv
-    case label_absurd hb ha => cases ha
-  case cinstr hb => apply! csingleton _ .var
-  case cbound hb => apply! cbound _ .var
-  case singleton_proj_sub hk =>
-    rw [← CaptureSet.proj_singleton] at hsc
-    apply! hsc.subkind
-  case singleton_proj_l => apply! hsc.proj
-  case singleton_proj C K hs ih =>
-    generalize h : C.proj K = D at hsc
+    case absurd he => apply! absurd_set
+  case cinstr hb => apply! csingleton
+  case cbound hb => apply! cbound
+  case subkind => apply! hsc.subkind_singleton
+  case proj_absurd he => apply! absurd
+  case proj_split =>
     cases hsc
-    case empty =>
-      unfold CaptureSet.proj at h; split at h <;> simp at h
-      rw [← CaptureSet.proj_singleton]; apply proj; apply ih .empty
-    case union iha ihb =>
-      unfold CaptureSet.proj at h; split at h <;> simp at h
-      have ⟨_, _⟩ := h; subst_vars; simp_all
-
-
-
-
-
-
-
-
-
-
-
-
-
-
-
-
-
-
-
--- theorem WellScoped.capture_kind (hsc : WellScoped Γ cont (C.proj K)) (hk : Γ ⊢ C :k K) : WellScoped Γ cont C := by
---   induction hk
---   case var hb hk ih =>
---     cases hsc
---     case proj_singleton hsc hs =>
---       cases hs
---       rename_i hs
---       cases hs
---       assumption
---     case label_disj hb1 hd hsp =>
---       cases hsp
---       case here hs =>
---         cases hs
---         cases Context.bound_lbound_absurd hb hb1
---       case there hsp => cases hsp
---   case cvar hb => apply! ckind
---   case cbound hb hk ih =>
---     cases hsc
---     case proj_singleton hsc hs =>
---       cases hs
---       rename_i hs
---       cases hs
---       assumption
---     case label_disj hsp =>
---       cases hsp
---       case here hs _ => cases hs
---       case there hsp => cases hsp
---   case cinstr hb hk ih =>
---     cases hsc
---     case proj_singleton hsc hs =>
---       cases hs
---       rename_i hs
---       cases hs
---       assumption
---     case label_disj hsp =>
---       cases hsp
---       case here hs _ => cases hs
---       case there hsp => cases hsp
---   case sub hsk hk ih =>
---     apply! ih $ hsc.subkind _
---   case empty => apply! empty
---   case singleton_proj_kind =>
---     cases hsc
---     case proj_singleton hsc hs =>
---       cases hs
---       rename_i hs
---       cases hs
---       apply! proj_singleton hsc $ .proj _
---     case label_disj hb hd hsp =>
---       cases hsp
---       case here hs =>
---         cases hs
---         apply! label_disj hb hd $ .here _
---       case there hsp =>
---         apply! label_disj
---   case singleton_proj hk ih =>
---     cases hsc
---     case proj_singleton hsc hs =>
---       cases hs
---       apply! proj_singleton hsc
---     case label_disj hb hd hsp =>
---       cases hsp
---       case here hs =>
---         cases hs
---         rename_i hs
---         have h := label_disj hb hd (.here hs) (cont:=cont)
---         have h1 := ih h
---         apply h1.proj
---       case there hsp => apply! label_disj
---   -- case singleton_proj_disj hk hd ih =>
---   --   cases hsc
---   --   case proj_singleton hsc hs =>
---   --     cases hs
---   --     apply! proj_singleton
---   --   case label_disj hb hd hsp =>
---   --     cases hsp
---   --     case here hs =>
---   case union ha hb iha ihb =>
---     simp at hsc
---     cases hsc
---     apply! union (iha _) (ihb _)
-
--- theorem WellScoped.subcapt
---   (hsc : WellScoped Γ cont C)
---   (hs : Γ ⊢ C' <:c C) :
---   WellScoped Γ cont C' := by
---   induction hs
---   case trans ih1 ih2 => exact ih1 (ih2 hsc)
---   case subset hs => exact hsc.subset hs
---   case union ih1 ih2 => exact .union (ih1 hsc) (ih2 hsc)
---   case var hb => exact .singleton hb hsc
---   case cinstl hb1 =>
---     cases hsc
---     case csingleton hb =>
---       have h := Context.cbound_injective hb1 hb; injections; subst_vars
---       assumption
---     case cbound hb => cases Context.cbound_injective hb1 hb
---     case ckind hb => cases Context.cbound_injective hb1 hb
---     case label_disj hsp => cases hsp
---   case cinstr hb => exact .csingleton hb hsc
---   case cbound hb => exact .cbound hb hsc
---   case singleton_proj_sub hs =>
---     rename_i s K1 K2
---     have h : (CaptureSet.singleton (s.proj K2)) = (CaptureSet.singleton s).proj K2 := by simp
---     rw [h] at hsc
---     exact hsc.subkind hs
---   case singleton_proj_l => exact hsc.proj
---   case proj_r C D K hs hk ih =>
---     cases hk
---     case cvar => apply! ckind
---     case var hb hk =>
-
---       sorry
---     case cbound => sorry
---     case cinstr => sorry
---     case sub => sorry
---     case empty => sorry
---     case singleton_proj_kind => sorry
---     case singleton_proj => sorry
---     -- case singleton_proj_disj => sorry
---     case union => sorry
---   case singleton_proj_disj hd hk => sorry
--- -- termination_by?
-
--- -- theorem WellScoped.subkind
-
--- -- theorem WellScoped.var_inv
--- --   (hsc : WellScoped Γ cont {x=x})
--- --   (hbx : Γ.Bound x (S^C)) :
--- --   WellScoped Γ cont C := by
--- --   cases hsc
--- --   case singleton =>
--- --     rename_i hbx'
--- --     have h := Context.bound_injective hbx hbx'
--- --     cases h
--- --     trivial
--- --   case label =>
--- --     exfalso
--- --     apply Context.bound_lbound_absurd <;> easy
-
--- -- theorem WellScoped.label_inv
--- --   (hsc : WellScoped Γ cont {x=x})
--- --   (hbl : Γ.LBound x S) :
--- --   ∃ tail, cont.HasLabel x tail := by
--- --   cases hsc
--- --   case singleton =>
--- --     exfalso
--- --     apply Context.bound_lbound_absurd <;> easy
--- --   case label => aesop
+    apply! proj_merge_singleton
+  case proj_merge =>
+    have h1 := hsc.subkind_singleton .union_rl
+    have h2 := hsc.subkind_singleton .union_rr
+    apply! union
 
 end Capless
